First version of model with sentry capabilities
Currently only guarantees monotonicity if sentries are never invoked,
but it should be possible to relax that to allow jumps to sentries
within the compartment.

model/Capabilities_lemmas.thy
@@ -23,6 +23,10 @@ inductive_set derivable :: "'cap set \<Rightarrow> 'cap set" for C :: "'cap set"
     "\<lbrakk>c' \<in> derivable C; c'' \<in> derivable C; is_tagged_method CC c'; is_tagged_method CC c'';
       \<not>is_sealed_method CC c''; \<not>is_sealed_method CC c'; permits_seal_method CC c''\<rbrakk> \<Longrightarrow>
      seal CC c' (get_cursor_method CC c'') \<in> derivable C"
+| SealEntry:
+    "\<lbrakk>c' \<in> derivable C; \<not>is_sealed_method CC c'; permits_execute_method CC c';
+      is_sentry_method CC (seal CC c' otype)\<rbrakk> \<Longrightarrow>
+     seal CC c' otype \<in> derivable C"
 
 lemma leq_cap_refl[simp, intro]:
   "leq_cap CC c c"
@@ -131,6 +135,12 @@ next
     then have "cap_derivable_bounded CC (Suc (max n' n'')) C (seal CC c' (get_cursor_method CC c''))"
       using Seal.hyps
       by auto
+    then show ?case by blast
+  next
+    case (SealEntry c' otype)
+    then obtain n where "cap_derivable_bounded CC n C c'"
+      by blast
+    then have "cap_derivable_bounded CC (Suc n) C (seal CC c' otype)" using SealEntry.hyps by auto
     then show ?case by blast
   qed
   then show "cap_derivable CC C c" by (simp add: cap_derivable_def)
