model/Cheri_axioms_lemmas.thy
@@ -233,6 +233,25 @@ lemma load_mem_axiomE:
   unfolding load_mem_axiom_def
   by blast
 
+lemma store_cap_reg_axiomE:
+  assumes "store_cap_reg_axiom CC ISA has_ex invoked_caps t"
+    and "writes_to_reg_at_idx i t = Some r"
+    and "c \<in> writes_reg_caps_at_idx CC ISA i t"
+  obtains (Derivable) "cap_derivable CC (available_caps CC ISA i t) c"
+  | (Ex) has_ex and "r \<in> PCC ISA"
+    and "c \<in>  exception_targets ISA {v'. \<exists>r' j. j < i \<and> index t j = Some (E_read_reg r' v') \<and> r' \<in> KCC ISA}"
+  | (Sentry) cs where "c \<in> invoked_caps" and "cap_derivable CC (available_caps CC ISA i t) cs"
+    and "is_sentry_method CC cs" and "is_sealed_method CC cs"
+    and "leq_cap CC c (unseal CC cs True)" and "r \<in> PCC ISA"
+  | (CCall) cc cd where "c \<in> invoked_caps"
+    and "cap_derivable CC (available_caps CC ISA i t) cc"
+    and "cap_derivable CC (available_caps CC ISA i t) cd"
+    and "invokable CC cc cd"
+    and "(leq_cap CC c (unseal CC cc True) \<and> r \<in> PCC ISA) \<or> (leq_cap CC c (unseal CC cd True) \<and> r \<in> IDC ISA)"
+  using assms
+  unfolding store_cap_reg_axiom_def
+  by blast
+
 (*lemma store_cap_reg_axiom_invoked_caps_mono:
   fixes invoked_caps :: "('cap \<times> 'cap) set"
   assumes "store_cap_reg_axiom CC ISA has_ex invoked_caps t"
